Refactor interface monad

src/examples/parser_entry.lean
@@ -2,42 +2,18 @@ import interface
 open lean.parser
 open interactive
 
-meta def main_tactic : tactic unit := do
-  ts <- get_state,
-  let init_search_state := search_state.new ts,
-  server_loop.run init_search_state,
-  return ()
-
-meta def parse_string (ps : lean.parser_state) (s : string) : tactic pexpr :=
-match (lean.parser.with_input interactive.types.texpr s) ps with
-| (interaction_monad.result.exception error ref s') := tactic.failed
-| (interaction_monad.result.success a s) := return a.1
-end
-
-meta def set_new_goal1 (goal : pexpr) : tactic unit :=
-do
-  e <- tactic.to_expr goal,
-  v <- tactic.mk_meta_var e,
-  tactic.set_goals [v],
-  return ()
-
-meta def get_parser_state : lean.parser lean.parser_state :=
-λ ps, interaction_monad.result.success ps ps
+-- set up server
+meta def server : json_server lean_server_request lean_server_response := {
+  get_line := io.get_line,    -- communicate via stdin
+  put_line := io.put_str_ln,  -- communicate via stdout
+  get_json := json_server.get_custom_json,   -- use custom format since faster
+  put_json := json_server.put_standard_json, -- use standard format  
+}
 
 @[user_command]
-meta def parse_for_me_cmd (meta_info : interactive.decl_meta_info) (_ : interactive.parse (tk "parse_for_me")) : lean.parser unit :=
-do e <- interactive.types.texpr,
-   ps <- get_parser_state,
-   lean.parser.of_tactic $ do
-     let s := "foo + 10 = 20",
-     pexp <- parse_string ps s,
-     set_new_goal1 pexp,
-     tactic.trace_state,
-     main_tactic
+meta def run_interface_with_goal_cmd (meta_info : interactive.decl_meta_info) (_ : interactive.parse (tk "run_interface_with_goal")) : lean.parser unit :=
+do goal <- interactive.types.texpr,
+  run_interface_from_parser server goal
 .
 
---parse_for_me true .  -- will fail since can't access foo
-
-def foo := 1
-
-parse_for_me true . -- will succeed
+run_interface_with_goal 1 + 1 = 2 . -- will succeed
