src/interface.lean
@@ -1,5 +1,5 @@
 import system.io
-import tactic.core  -- for get_state, set_state
+import tactic.core  -- TODO: Remove this but need derive handler for monad
 import tools.serialization -- TODO: Serialize Lean's standard raw expression format
 import tools.json
 import tools.json_server
@@ -10,97 +10,209 @@ import api_classes
 open io
 
 /-
-meta def tactic.to_ex {α : Type} (t : tactic α) : tactic (exceptional α) :=
-λ s, match t s with
-| (interaction_monad.result.exception (some fmt) ref s') := interaction_monad.result.success (exceptional.exception (λ _, fmt ())) s
-| (interaction_monad.result.exception none ref s') := interaction_monad.result.success (exceptional.fail "") s
-| (interaction_monad.result.success a s) := interaction_monad.result.success (exceptional.success a) s
-end
--/
+The interface monad is made of three parts
+- A read-only configuration structure having  
+  information on how to communicate with io and the parser as
+  well as other read-only information.
+- A "mutable" search-state datastructure which is used for keeping
+  track of all the tactic states visited.  (When this monad calls a tactic
+  it will do so explicitly by specifying the tactic_state to use.)
+- An except output with many types of exceptions indicating various types
+  of failures, which can be handled differently.
+-/  
 
--- Data structures
-meta structure search_state :=
-(tactic_states : list tactic_state)
-(current_state_ix : nat)
+/- A read-only configuration structure having information on how to 
+  communicate with io and the parser as well as other read-only information. -/
+meta structure interface_config :=
+/- Specifies how to communicate with an external process and what protocal to
+use to pass json-like information. -/
+(server : json_server lean_server_request lean_server_response)
+/- An optional parser state.  This can only be gotten from running the 
+interface through a parser, but it allows the external process to communicate
+goals via lean syntax instead of more combersome methods. -/
+(ps : option lean.parser_state := none)
+/- The initial tactic state, used to seed the search_state. -/
+(initial_ts : tactic_state)
 
-meta def search_state.size (state : search_state) : nat := state.tactic_states.length
+/- A persistant search state data structure which is used for keeping
+  track of all the tactic states visited.  (When this monad calls a tactic
+  it will do so explicitly by specifying the tactic_state to use.) -/
+meta structure interface_state :=
+(tactic_states : list tactic_state)  -- if not fast enough, use a better lookup data structure
+(current_ts_ix : nat) -- TODO: Remove after new API
 
-meta def search_state.get (n : nat) (state : search_state) : option tactic_state :=
-if n < state.tactic_states.length then 
-  state.tactic_states.nth (state.tactic_states.length - n - 1) 
+meta def interface_state.initialize (ts : tactic_state) : interface_state := 
+{ tactic_states := [ts], current_ts_ix := 0 }
+
+meta def interface_state.size (state : interface_state) : nat := 
+state.tactic_states.length
+
+meta def interface_state.get (ix : nat) (state : interface_state) : option tactic_state :=
+if ix < state.tactic_states.length then 
+  state.tactic_states.nth (state.tactic_states.length - ix - 1) 
 else 
   none
 
-meta def search_state.put (state : search_state) (s : tactic_state) : search_state :=
-⟨s :: state.tactic_states, state.size⟩ 
+meta def interface_state.put (state : interface_state) (ts : tactic_state) : interface_state × nat :=
+({ tactic_states := ts :: state.tactic_states, current_ts_ix := state.size }, state.size)
 
-meta def search_state.new (initial_state : tactic_state) : search_state :=
-⟨[initial_state], 0⟩
+-- TODO: Remove after new API
+meta def interface_state.set_current (state : interface_state) (ix : nat) : option interface_state :=
+if ix < state.tactic_states.length then 
+  some { tactic_states := state.tactic_states, current_ts_ix := ix }
+else 
+  none
 
+/- Many types of exceptions indicating various types of failures, which can be 
+handled differently. -/
 meta inductive interface_ex
 | tactic_exception (error : option (unit → format))
+| parser_exception (error : option (unit → format))
+| io_exception (error : option (unit → format))
 | apply_tactic_exception (error : option (unit → format))
 | user_input_exception (msg : string)
-| other
--- add more as needed
+| unexpected_error (msg : string)
+| other -- TODO: This is a placeholder.  Don't use
+-- TODO: Add more as needed.
 
 
--- TODO: Add server stuff as part of the interface monad as a reader
--- TODO: Add parser state as a reader as well
--- TODO: Don't extend tactic state (pass state to run_tactic explicitly)
 
--- need to put the except_t inside the state_t for the desired backtracking properties
+-- need to put the except inside the state_t for the desired backtracking properties
 @[derive [monad]]
-meta def interface_m (α : Type) : Type := state_t search_state (except_t interface_ex tactic) α 
+meta def interface_m (α : Type) : Type := reader_t interface_config (state_t interface_state (except interface_ex)) α 
 
-meta def interface_m.run {α : Type} (m : interface_m α) (s : search_state) : tactic (except interface_ex (α × search_state)) := 
-(state_t.run m s).run
+-- show that interface_m is monad_except.  Don't know why this can't be done automatically.
+meta def interface_m.throw {α : Type} (e : interface_ex) : interface_m α := do
+reader_t.lift $ state_t.lift $ except.error e
 
-meta def get_search_state : interface_m search_state := state_t.get
-
-meta def put_search_state (s : search_state) : interface_m unit := state_t.put s
-
-
-/- Catch the error inside a tactic and convert to an except exception -/
-private meta def catch_errors {α : Type} (t : tactic α) : tactic (except interface_ex α) :=
-λ s, match t s with
-| (interaction_monad.result.exception error ref s') := interaction_monad.result.success (except.error (interface_ex.tactic_exception error)) s
-| (interaction_monad.result.success a s)  := interaction_monad.result.success (except.ok a) s
+meta def interface_m.catch {α : Type} (ma : interface_m α) (handle : interface_ex → interface_m α) : interface_m α :=
+reader_t.mk $ λ config, state_t.mk $ λ state,
+match (ma.run config).run state with
+| except.error e := ((handle e).run config).run state
+| e := e
 end
-
-private meta def lift_to_ex {α : Type} (t : tactic α) : except_t interface_ex tactic α := do
-e_a <- except_t.lift (catch_errors t),
-match e_a with
-| except.ok a := return a
-| except.error e := throw e
-end
-
-/- Lift tactic to interface_m and convert tactic failures to except.error (tactic_exception _) -/
-meta def interface_m.run_tactic {α : Type} (t : tactic α) : interface_m α :=
-state_t.lift (lift_to_ex t)
-
--- for some reason this is only automatically derived if I use the raw combinators
-meta def interface_m.throw {α : Type} (e : interface_ex) : state_t search_state (except_t interface_ex tactic) α := do
-throw e
-
--- for some reason this is only automatically derived if I use the raw combinators
-meta def interface_m.catch {α : Type} (ma : state_t search_state (except_t interface_ex tactic) α) (handle : interface_ex → state_t search_state (except_t interface_ex tactic) α) : state_t search_state (except_t interface_ex tactic) α := do
-catch ma handle
 
 meta instance interface_m_monad_except : monad_except interface_ex interface_m :=
 { throw := @interface_m.throw, catch := @interface_m.catch }
 
+-- reader/state monad stuff
+meta def interface_m.read_config : interface_m interface_config := reader_t.read
+meta def interface_m.get_state : interface_m interface_state := reader_t.lift state_t.get
+meta def interface_m.put_state (s : interface_state) : interface_m unit := reader_t.lift (state_t.put s)
+
+-- running tactic, parser, and io monads
+
+/- Run tactic and convert tactic failures to except.error (tactic_exception _) -/
+meta def interface_m.run_tactic {α : Type} (ts : tactic_state) (t : tactic α) : interface_m (α × tactic_state) :=
+match t ts with
+| (interaction_monad.result.exception error ref ts') := throw (interface_ex.tactic_exception error)
+| (interaction_monad.result.success a ts')  := return (a, ts')
+end
+
+/- Run tactic and throw away the new tactic state -/
+meta def interface_m.run_tactic1 {α : Type} (ts : tactic_state) (t : tactic α) : interface_m α :=
+do (a, _) <- interface_m.run_tactic ts t, return a
+
+/- Run tactic and return only the tactic state -/
+meta def interface_m.run_tactic2 {α : Type} (ts : tactic_state) (t : tactic α) : interface_m tactic_state :=
+do (_, ts) <- interface_m.run_tactic ts t, return ts
+
+/- Run the parser on a string -/
+meta def interface_m.parse_string (ps : lean.parser_state) (s : string) : interface_m pexpr :=
+match (lean.parser.with_input interactive.types.texpr s) ps with
+| (interaction_monad.result.exception error ref s') := throw (interface_ex.parser_exception error)
+| (interaction_monad.result.success a s) := return a.1
+end
+
+/- Run io monad
+(Need a tactic state as an entry point.  I don't think it matters which one.) -/
+meta def interface_m.run_io {α : Type} (ts : tactic_state) (i : io α) : interface_m α :=
+match (tactic.unsafe_run_io i) ts with
+| (interaction_monad.result.exception error ref ts') := throw (interface_ex.io_exception error)
+| (interaction_monad.result.success a ts') := return a
+end
+
+/- Run this monad and return an except object.
+It doesn't take an interface_state, which is instead seeded by the config.initial_ts. 
+We don't return the final state, just the value of type α. -/
+meta def interface_m.run {α : Type} (m : interface_m α) (config : interface_config) : except interface_ex α := 
+let state := interface_state.initialize config.initial_ts in
+((reader_t.run m config).run state).map(λ as, as.1)
 
 
--- set up server
-meta def server : json_server lean_server_request lean_server_response := {
-  get_line := io.get_line,    -- communicate via stdin
-  put_line := io.put_str_ln,  -- communicate via stdout
-  get_json := json_server.get_custom_json,   -- use custom format since faster
-  put_json := json_server.put_standard_json, -- use standard format  
-}
+-- TODO: Move this elsewhere
+/-
 
--- manipulating the tactic state and the search state
+-/
+
+namespace interface_m
+
+-- abstractions for accessing config and state and modifying state
+
+meta def get_tactic_state (ix : nat): interface_m tactic_state := do
+state <- get_state,
+match state.get(ix) with
+| some ts := return ts
+| none := throw $ interface_ex.user_input_exception $ "No state index " ++ repr(ix)
+end
+
+/- This is tactic state from the config used to initialize the monad -/
+meta def get_inital_tactic_state : interface_m tactic_state := do
+config <- read_config,
+return config.initial_ts
+
+-- TODO: Remove after new API
+meta def get_current_tactic_state : interface_m tactic_state := do
+state <- get_state,
+match state.get(state.current_ts_ix) with
+| some ts := return ts
+| none := throw $ interface_ex.unexpected_error $ "BUG: Current state index " ++ repr(state.current_ts_ix) ++ " has not corresponding state."
+end
+
+-- TODO: Remove after new API
+meta def set_tactic_state (ix : nat): interface_m unit := do
+state <- get_state,
+match state.set_current ix with
+| some s := put_state s
+| none := throw $ interface_ex.user_input_exception $ "No state index " ++ repr(ix)
+end
+
+-- TODO: Remove after new API
+meta def get_current_tactic_state_ix : interface_m nat := do
+state <- get_state,
+return state.current_ts_ix
+
+meta def register_tactic_state (ts : tactic_state) : interface_m nat := do
+state <- get_state,
+let (state, ix) := state.put ts,
+put_state state,
+return ix
+
+meta def reset_all_tactic_states (ts0 : tactic_state) : interface_m unit := do
+put_state (interface_state.initialize ts0)
+
+meta def read_io_request : interface_m lean_server_request := do
+config <- read_config,
+let server := config.server,
+let ts0 := config.initial_ts, -- run io from initial tactic_state.  I don't think it matters which one I use.
+interface_m.run_io ts0 server.get_request
+
+meta def write_io_response (response: lean_server_response) : interface_m unit := do
+config <- read_config,
+let server := config.server,
+let ts0 := config.initial_ts,
+interface_m.run_io ts0 (server.send_response response)
+
+meta def debug (msg : string) : interface_m unit := do
+config <- read_config,
+let ts0 := config.initial_ts,
+interface_m.run_tactic1 ts0 (tactic.trace msg)
+
+end interface_m
+
+
+-- TODO: Split into two or three files (monad, repl, entry points)
+-- read eval print
 
 meta def deserialize_expr (sexpr : string) : interface_m expr :=
 match (expr.deserialize sexpr) with
@@ -108,53 +220,14 @@ match (expr.deserialize sexpr) with
 | (sum.inr h) := return h
 end
 
-meta def set_new_goal (goal : expr) : interface_m unit :=
-interface_m.run_tactic $ do
-  v <- tactic.mk_meta_var goal,
-  tactic.set_goals [v],
-  return ()
-
-meta def set_tactic_state (tactic_state_index : nat) : interface_m unit := do
-states <- get_search_state,
-match states.get tactic_state_index with
-| some s := interface_m.run_tactic (set_state s)
-| none := throw (interface_ex.user_input_exception "State index out of bounds")
-end,
-put_search_state { 
-  tactic_states := states.tactic_states, 
-  current_state_ix := tactic_state_index 
-}
-
-meta def register_tactic_state : interface_m unit := do
-s <- interface_m.run_tactic get_state,
-states <- get_search_state,
-put_search_state (states.put s)
-
-meta def get_tactic_state_ix : interface_m nat := do
-states <- get_search_state,
-return states.current_state_ix
-
-meta def reset_all_tactic_states : interface_m unit := do
-s <- interface_m.run_tactic get_state,
-put_search_state (search_state.new s)
-
-
-
-
--- read eval print
-
-meta def read_user_request : interface_m lean_server_request :=
-interface_m.run_tactic (tactic.unsafe_run_io server.get_request)
-
-
-
-meta def apply_tactic (t : tactic unit): interface_m unit := 
-catch (interface_m.run_tactic t) $ λ e, match e with
+meta def apply_tactic (t : tactic unit): interface_m tactic_state := do
+ts <- interface_m.get_current_tactic_state,
+catch (interface_m.run_tactic2 ts t) $ λ e, match e with
 | interface_ex.tactic_exception error := throw (interface_ex.apply_tactic_exception error)
 | e := throw e
 end
 
-meta def apply_tactic_request : lean_tactic -> interface_m unit
+meta def apply_tactic_request (ts : tactic_state) : lean_tactic -> interface_m tactic_state
 | (lean_tactic.apply sexpr) := do
   h <- deserialize_expr sexpr,
   apply_tactic (tactic.interactive.concat_tags (tactic.apply h))
@@ -166,18 +239,22 @@ meta def apply_tactic_request : lean_tactic -> interface_m unit
 | lean_tactic.left := apply_tactic (tactic.interactive.left)
 | lean_tactic.right := apply_tactic (tactic.interactive.right)
 
+meta def mk_new_goal (ts0 : tactic_state) (goal : expr) : interface_m tactic_state := do
+interface_m.run_tactic2 ts0 $ (do
+  v <- tactic.mk_meta_var goal,
+  tactic.set_goals [v],
+  return ()
+)
+
 meta def change_goal (sexp : string) : interface_m unit := do
   goal_expr <- deserialize_expr sexp,
-  set_new_goal goal_expr,
-  reset_all_tactic_states,
-  register_tactic_state
-
-meta def jump_to_tactic_state (state_index : nat) : interface_m unit := do
-  set_tactic_state state_index
+  ts0 <- interface_m.get_inital_tactic_state,
+  ts <- mk_new_goal ts0 goal_expr,
+  interface_m.reset_all_tactic_states ts
 
 meta def change_state : lean_state_control -> interface_m unit
 | (lean_state_control.jump_to_state state_index) := 
-  set_tactic_state state_index
+  interface_m.set_tactic_state state_index
 | (lean_state_control.change_top_goal sexp) := 
   change_goal sexp
 
@@ -200,15 +277,15 @@ s1 <- (do
 ) <|> (return s),
 return s1
 
-meta def get_state_info : interface_m string := do
-current_state_ix <- get_tactic_state_ix,
-interface_m.run_tactic (state_info_str current_state_ix)
+meta def get_state_info (ts : tactic_state) (ix : nat): interface_m string := do
+interface_m.run_tactic1 ts (state_info_str ix)
 
 meta def eval_user_request : lean_server_request → interface_m lean_server_response
 | (lean_server_request.apply_tactic tac) := catch (do
-    apply_tactic_request tac,
-    register_tactic_state,
-    state_info <- get_state_info,
+    ts <- interface_m.get_current_tactic_state,
+    ts <- apply_tactic_request ts tac,
+    ix <- interface_m.register_tactic_state ts,
+    state_info <- get_state_info ts ix,
     let msg := "Tactic succeeded:" ++ "\n" ++ state_info,
     let result := lean_tactic_result.success msg,
     let response := lean_server_response.apply_tactic result,
@@ -239,8 +316,9 @@ meta def eval_user_request : lean_server_request → interface_m lean_server_res
   end
 | (lean_server_request.change_state state_control) := catch (do
     change_state state_control,
-    register_tactic_state,
-    state_info <- get_state_info,
+    ts <- interface_m.get_current_tactic_state,
+    ix <- interface_m.get_current_tactic_state_ix,
+    state_info <- get_state_info ts ix,
     let msg := "state change succeeded:" ++ "\n" ++ state_info,
     let result := lean_state_result.success msg,
     let response := lean_server_response.change_state result,
@@ -262,13 +340,10 @@ meta def eval_user_request : lean_server_request → interface_m lean_server_res
   | e := throw e
   end
 
-meta def write_response (response: lean_server_response) : interface_m unit :=
-interface_m.run_tactic $ tactic.unsafe_run_io (server.send_response response)
-
 meta def server_loop : interface_m unit := do
 response <- catch (do 
   -- TODO: Might want to split into errors that are parsing errors (json type things) and ones that are bugs on my end
-  request <- read_user_request,
+  request <- interface_m.read_io_request,
   eval_user_request request
 ) (λ e, 
   match e with
@@ -282,5 +357,45 @@ response <- catch (do
   | e := throw e 
   end
 ),
-write_response response,
+interface_m.write_io_response response,
 server_loop
+
+-- commands for running the interface
+-- TODO: maybe it is better not to have the initial tactic state inside the config
+--       so that the config can be made ahead of time
+meta def run_interface_from_tactic (server : json_server lean_server_request lean_server_response) : tactic (except interface_ex unit) := do
+  ts <- get_state,
+  let config : interface_config := {
+    server := server,
+    ps := none,
+    initial_ts := ts
+  },
+  -- it is very important that we do something with server_loop.run config 
+  -- (like return it) otherwise it won't be run
+  return $ server_loop.run config
+  
+meta def get_parser_state : lean.parser lean.parser_state :=
+λ ps, interaction_monad.result.success ps ps
+
+meta def tactic_state_at_goal (goal : pexpr) : lean.parser tactic_state :=
+lean.parser.of_tactic $ do
+  e <- tactic.to_expr goal,
+  v <- tactic.mk_meta_var e,
+  tactic.set_goals [v],
+  ts <- get_state,
+  return ts
+
+meta def run_interface_from_parser (server : json_server lean_server_request lean_server_response) (goal : pexpr) : lean.parser unit := do
+  ps <- get_parser_state,
+  ts <- tactic_state_at_goal goal,
+  let config : interface_config := {
+    server := server,
+    ps := ps,
+    initial_ts := ts
+  },
+  let ts := server_loop.run config,
+  return ()
+
+meta def run_interface_from_io (server : json_server lean_server_request lean_server_response): io unit := do
+  io.run_tactic (run_interface_from_tactic server),
+  return ()
